refactor: rework monads & exception handling

ffi/nerodia.c
@@ -155,21 +155,17 @@ LEAN_EXPORT lean_obj_res nerodia_py_object_ctx(b_lean_obj_arg self) {
   return lean_alloc_external(g_py_context_external_class, pctx);
 }
 
+LEAN_EXPORT lean_obj_res nerodia_py_context_mk_object(lean_obj_arg ctx, size_t ptr) {
+  return nerodia_of_object((PyObject*)ptr, ctx);
+}
+
 LEAN_EXPORT lean_obj_res nerodia_py_context_clear_error(b_lean_obj_arg ctx) {
   PyErr_Clear();
   return lean_box(0);
 }
 
-LEAN_EXPORT lean_obj_res nerodia_py_context_get_raised_exception(lean_obj_arg ctx) {
-  PyObject *ex = PyErr_GetRaisedException();
-  if (ex) {
-    lean_obj_res r = lean_alloc_ctor(1, 1, 0);
-    lean_ctor_set(r, 0, nerodia_of_object(ex, ctx));
-    return r;
-  } else {
-    lean_dec_ref(ctx);
-    return lean_box(0);
-  }
+LEAN_EXPORT size_t nerodia_get_raised_exception() {
+  return (size_t)PyErr_GetRaisedException();
 }
 
 LEAN_EXPORT lean_obj_res nerodia_py_context_none(lean_obj_arg ctx) {
@@ -202,9 +198,8 @@ LEAN_EXPORT lean_obj_res nerodia_py_context_str_type(lean_obj_arg ctx) {
 
 /* ### Type Objects */
 
-LEAN_EXPORT lean_obj_res nerodia_py_type_object_get_qual_name(b_lean_obj_arg self, lean_obj_arg ctx) {
-  // TODO: handle potential errors here (allocation and static type name decode)
-  return nerodia_of_object(PyType_GetQualName(nerodia_to_type_object(self)), ctx);
+LEAN_EXPORT size_t nerodia_py_type_object_get_qual_name(b_lean_obj_arg self, b_lean_obj_arg ctx) {
+  return (size_t)PyType_GetQualName(nerodia_to_type_object(self));
 }
 
 LEAN_EXPORT uint8_t nerodia_py_type_object_is_heap_type(b_lean_obj_arg self) {
@@ -217,73 +212,49 @@ LEAN_EXPORT uint8_t nerodia_py_type_object_is_immutable(b_lean_obj_arg self) {
 
 /** ### Strings */
 
-LEAN_EXPORT lean_obj_res nerodia_mk_string(b_lean_obj_arg s, lean_obj_arg ctx) {
+/* mkPyStrObject : @& String -> BaseIO (CPtr PyStrObject) */
+LEAN_EXPORT size_t nerodia_mk_py_str_object(b_lean_obj_arg s) {
   // Lean strings include a null-terminator.
   // `FromStringAndSize` does not expect one, so use `size-1`.
   // Lean guarantees that the string is properly UTF-8 encoded.
-  // TODO: handle potential allocation errors here
-  PyObject * o = PyUnicode_FromStringAndSize(lean_string_cstr(s), lean_string_size(s)-1);
-  return nerodia_of_object(o, ctx);
+  return (size_t)PyUnicode_FromStringAndSize(
+    lean_string_cstr(s), lean_string_size(s)-1);
 }
 
-/* str : PyObject -> PyContext -> BaseIO (Option PyStrObject) */
-LEAN_EXPORT lean_obj_res nerodia_py_object_str(b_lean_obj_arg o, lean_obj_arg ctx) {
-  PyObject * s = PyObject_Str(nerodia_to_object(o));
-  if (s) {
-    lean_object * r = lean_alloc_ctor(1, 1, 0);
-    lean_ctor_set(r, 0, nerodia_of_object(s, ctx));
-    return r;
-  } else {
-    lean_dec_ref(ctx);
-    return lean_box(0);
-  }
+/* str : @& PyObject -> BaseIO (CPtr PyStrObject) */
+LEAN_EXPORT size_t nerodia_py_object_str(b_lean_obj_arg o) {
+  return (size_t)PyObject_Str(nerodia_to_object(o));
 }
 
-/* repr : PyObject -> PyContext -> BaseIO (Option PyStrObject) */
-LEAN_EXPORT lean_obj_res nerodia_py_object_repr(b_lean_obj_arg o, lean_obj_arg ctx) {
-  PyObject * s = PyObject_Repr(nerodia_to_object(o));
-  if (s) {
-    lean_object * r = lean_alloc_ctor(1, 1, 0);
-    lean_ctor_set(r, 0, nerodia_of_object(s, ctx));
-    return r;
-  } else {
-    lean_dec_ref(ctx);
-    return lean_box(0);
-  }
+/* repr : @& PyObject -> BaseIO (CPtr PyStrObject) */
+LEAN_EXPORT size_t nerodia_py_object_repr(b_lean_obj_arg o) {
+  return (size_t)PyObject_Repr(nerodia_to_object(o));
 }
 
-/* getString : PyStrObject -> PyContext -> BaseIO (Option String) */
-LEAN_EXPORT lean_obj_res nerodia_py_str_object_get_string(b_lean_obj_arg o, lean_obj_arg ctx) {
+/* toString : @& PyStrObject -> String */
+LEAN_EXPORT lean_obj_res nerodia_py_str_object_to_string(b_lean_obj_arg o) {
   Py_ssize_t size;
   const char * cs = PyUnicode_AsUTF8AndSize(nerodia_to_object(o), &size);
   if (LEAN_LIKELY(cs != NULL)) {
     // Both Lean and `AsUTF8AndSize` have a null terminator,
     // but neither include it in `size`
-    lean_obj_res s = lean_mk_string_from_bytes_unchecked(cs, size);
-    lean_dec_ref(ctx);
-    lean_obj_res r = lean_alloc_ctor(1, 1, 0);
-    lean_ctor_set(r, 0, s);
-    return r;
+    return lean_mk_string_from_bytes_unchecked(cs, size);
+  } else if (PyErr_ExceptionMatches(PyExc_MemoryError)) {
+    lean_internal_panic_out_of_memory();
   } else {
-    lean_dec_ref(ctx);
-    return lean_box(0);
+    // It should be impossible for the encode to fail
+    // except in the case of memory errors
+    PyErr_WriteUnraisable(NULL);
+    lean_internal_panic_unreachable();
   }
 }
 
-/* decoeUtf8 : PyStrObject -> PyContext -> BaseIO (Option PyBytesObjects) */
-LEAN_EXPORT lean_obj_res nerodia_py_str_object_decode_utf8(b_lean_obj_arg o, lean_obj_arg ctx) {
-  PyObject * bytes = PyUnicode_AsUTF8String(nerodia_to_object(o));
-  if (bytes) {
-    lean_obj_res v = nerodia_of_object(bytes, ctx);
-    lean_obj_res r = lean_alloc_ctor(1, 1, 0);
-    lean_ctor_set(r, 0, v);
-    return r;
-  } else {
-    lean_dec_ref(ctx);
-    return lean_box(0);
-  }
+/* utf8Encode : @& PyStrObject -> BaseIO (CPtr PyBytesObjects) */
+LEAN_EXPORT size_t nerodia_py_str_object_utf8_encode(b_lean_obj_arg o) {
+  return (size_t)PyUnicode_AsUTF8String(nerodia_to_object(o));
 }
 
+/* toByteArray : @& PyBytesObject -> ByteArray */
 LEAN_EXPORT lean_obj_res nerodia_py_bytes_object_to_byte_array(b_lean_obj_arg self) {
   PyObject* o = nerodia_to_object(self);
   size_t sz = PyBytes_Size(o);
