lakefile.lean
@@ -4,6 +4,7 @@ open Lean (Json ToJson FromJson toJson fromJson?)
 
 package nerodia where
   leanOptions := #[⟨`doc.verso, true⟩]
+  buildType := .debug
 
 /-! ## Python -/
 
